WIP
WIP

WIP

WIP

WIP

WIP

WIP

Debugging

WIP

WIP

WIP

WIP

WIP

WIP

WIP

WIP

WIP

WIP

WIP

WIP

WIP

WIP

WIP

WIP

WIP

WIP

WIP

WIP

src/Reflection/InputSyntax.v
@@ -1,7 +1,7 @@
 (** * PHOAS Representation of Gallina which allows exact denotation *)
 Require Import Coq.Strings.String.
 Require Import Crypto.Reflection.Syntax.
-Require Import Crypto.Reflection.Relations.
+Require Import Crypto.Reflection.ExprInversion.
 Require Import Crypto.Reflection.InterpProofs.
 Require Import Crypto.Util.Tuple.
 Require Import Crypto.Util.Tactics.
@@ -16,14 +16,20 @@ Section language.
   Context (base_type_code : Type).
 
   Local Notation flat_type := (flat_type base_type_code).
-  Local Notation type := (type base_type_code).
+  Inductive type := Tflat (A : flat_type) | Arrow (A : flat_type) (B : type).
 
   Section expr_param.
     Context (interp_base_type : base_type_code -> Type).
     Context (op : flat_type (* input tuple *) -> flat_type (* output type *) -> Type).
-    Local Notation interp_type := (interp_type interp_base_type).
     Local Notation interp_flat_type_gen := interp_flat_type.
     Local Notation interp_flat_type := (interp_flat_type interp_base_type).
+
+    Fixpoint interp_type (t : type) :=
+      match t with
+      | Tflat A => interp_flat_type A
+      | Arrow A B => (interp_flat_type A -> interp_type B)%type
+      end.
+
     Section expr.
       Context {var : flat_type -> Type}.
 
@@ -36,9 +42,11 @@ Section language.
       | Pair : forall {t1}, exprf t1 -> forall {t2}, exprf t2 -> exprf (Prod t1 t2)
       | MatchPair : forall {t1 t2}, exprf (Prod t1 t2) -> forall {tC}, (var t1 -> var t2 -> exprf tC) -> exprf tC.
       Inductive expr : type -> Type :=
-      | Return {t} : exprf t -> expr t
-      | Abs {src dst} : (var (Tbase src) -> expr dst) -> expr (Arrow src dst).
-      Global Coercion Return : exprf >-> expr.
+      | Return {T} : exprf T -> expr (Tflat T)
+      | Abs {src dst} : (var src -> expr dst) -> expr (Arrow src dst).
+
+      Definition Fst {t1 t2} (v : exprf (Prod t1 t2)) : exprf t1 := MatchPair v (fun x y => Var x).
+      Definition Snd {t1 t2} (v : exprf (Prod t1 t2)) : exprf t2 := MatchPair v (fun x y => Var y).
     End expr.
 
     Definition Expr (t : type) := forall var, @expr var t.
@@ -57,7 +65,7 @@ Section language.
            end.
       Fixpoint interp {t} (e : @expr interp_flat_type t) : interp_type t
         := match e in expr t return interp_type t with
-           | Return _ x => interpf x
+           | Return _ v => interpf v
            | Abs _ _ f => fun x => @interp _ (f x)
            end.
 
@@ -67,6 +75,25 @@ Section language.
     Section compile.
       Context {var : base_type_code -> Type}
               (make_const : forall t, interp_base_type t -> op Unit (Tbase t)).
+
+      Fixpoint compilet (t : type) : Syntax.type base_type_code
+        := Syntax.Arrow
+             match t with
+             | Tflat T => Unit
+             | Arrow A (Tflat B) => A
+             | Arrow A B
+               => A * match compilet B with
+                      | Syntax.Arrow B' C' => B'
+                      end
+             end%ctype
+             match t with
+             | Tflat T => T
+             | Arrow A (Tflat B) => B
+             | Arrow A B
+               => match compilet B with
+                  | Syntax.Arrow B' C' => C'
+                  end
+             end.
 
       Fixpoint SmartConst (t : flat_type) : interp_flat_type t -> Syntax.exprf base_type_code op (var:=var) t
         := match t return interp_flat_type t -> Syntax.exprf _ _ t with
@@ -86,16 +113,40 @@ Section language.
            | MatchPair _ _ ex _ eC => Syntax.LetIn (@compilef _ ex) (fun xy => @compilef _ (eC (fst xy) (snd xy)))
            end.
 
-      Fixpoint compile {t} (e : @expr (interp_flat_type_gen var) t) : @Syntax.expr base_type_code op var t
-        := match e in expr t return @Syntax.expr _ _ _ t with
-           | Return _ x => Syntax.Return (compilef x)
-           | Abs a _ f => Syntax.Abs (fun x : var a => @compile _ (f x))
-           end.
+      (* ugh, so much manual annotation *)
+      Fixpoint compile {t} (e : @expr (interp_flat_type_gen var) t) : @Syntax.expr base_type_code op var (compilet t)
+        := match e in expr t return @Syntax.expr _ _ _ (compilet t) with
+           | Return _ v => Syntax.Abs (fun _ => compilef v)
+           | Abs src dst f
+             => let res := fun x => @compile _ (f x) in
+                match dst
+                      return (_ -> Syntax.expr _ _ (compilet dst))
+                             -> Syntax.expr _ _ (compilet (Arrow src dst))
+                with
+                | Tflat T
+                  => fun resf => Syntax.Abs (fun x => invert_Abs (resf x) tt)
+                | Arrow A B as dst'
+                  => match compilet dst' as cdst
+                           return (_ -> Syntax.expr _ _ cdst)
+                                  -> Syntax.expr _ _ (Syntax.Arrow
+                                                        (_ * match cdst with
+                                                             | Syntax.Arrow _ _ => _
+                                                             end)
+                                                        match cdst with
+                                                        | Syntax.Arrow _ _ => _
+                                                        end)
+                     with
+                     | Syntax.Arrow A' B'
+                       => fun resf => Syntax.Abs (fun x : interp_flat_type_gen var (_ * _)
+                                                  => invert_Abs (resf (fst x)) (snd x))
+                     end
+                end res
+               end.
     End compile.
 
     Definition Compile
                (make_const : forall t, interp_base_type t -> op Unit (Tbase t))
-               {t} (e : Expr t) : Syntax.Expr base_type_code op t
+               {t} (e : Expr t) : Syntax.Expr base_type_code op (compilet t)
       := fun var => compile make_const (e _).
 
     Section compile_correct.
@@ -126,33 +177,84 @@ Section language.
                  end.
       Qed.
 
-      Lemma Compile_correct {t} (e : @Expr t)
-      : interp_type_gen_rel_pointwise (fun _ => @eq _)
-                                      (Syntax.Interp interp_op (Compile make_const e))
-                                      (Interp interp_op e).
+      Lemma compile_flat_correct {T} (e : expr (Tflat T))
+      : forall x, Syntax.interp interp_op (compile make_const e) x = interp interp_op e.
+      Proof.
+        intros []; simpl.
+        let G := match goal with |- ?G => G end in
+        let G := match (eval pattern T, e in G) with ?G _ _ => G end in
+        refine match e in expr t return match t return expr t -> _ with
+                                        | Tflat T => G T
+                                        | _ => fun _ => True
+                                        end e
+               with
+               | Return _ _ => _
+               | Abs _ _ _ => I
+               end; simpl.
+        apply compilef_correct.
+      Qed.
+
+      Lemma Compile_flat_correct_flat {T} (e : Expr (Tflat T))
+        : forall x, Syntax.Interp interp_op (Compile make_const e) x = Interp interp_op e.
+      Proof. apply compile_flat_correct. Qed.
+
+      Lemma Compile_correct {src dst} (e : @Expr (Arrow src (Tflat dst)))
+      : forall x, Syntax.Interp interp_op (Compile make_const e) x = Interp interp_op e x.
       Proof.
         unfold Interp, Compile, Syntax.Interp; simpl.
         pose (e interp_flat_type) as E.
         repeat match goal with |- context[e ?f] => change (e f) with E end.
         clearbody E; clear e.
-        induction E.
-        { apply compilef_correct. }
-        { simpl; auto. }
+        let G := match goal with |- ?G => G end in
+        let G := match (eval pattern src, dst, E in G) with ?G _ _ _ => G end in
+        refine match E in expr t return match t return expr t -> _ with
+                                        | Arrow src (Tflat dst) => G src dst
+                                        | _ => fun _ => True
+                                        end E
+               with
+               | Abs src dst e
+                 => match dst
+                          return (forall e : _ -> expr dst,
+                                     match dst return expr (Arrow src dst) -> _ with
+                                     | Tflat dst => G src dst
+                                     | _ => fun _ => True
+                                     end (Abs e))
+                    with
+                    | Tflat _
+                      => fun e0 x
+                         => _
+                    | Arrow _ _ => fun _ => I
+                    end e
+               | Return _ _ => I
+               end; simpl.
+        refine match e0 x as e0x in expr t
+                     return match t return expr t -> _ with
+                            | Tflat _
+                              => fun e0x
+                                 => Syntax.interpf _ (invert_Abs (compile _ e0x) _)
+                                    = interp _ e0x
+                            | _ => fun _ => True
+                            end e0x
+               with
+               | Abs _ _ _ => I
+               | Return _ _ => _
+               end; simpl.
+        apply compilef_correct.
       Qed.
-
-      Lemma Compile_flat_correct {t : flat_type} (e : @Expr t)
-      : Syntax.Interp interp_op (Compile make_const e) = Interp interp_op e.
-      Proof. exact (@Compile_correct t e). Qed.
     End compile_correct.
   End expr_param.
 End language.
 
+Global Arguments Arrow {_} _ _.
+Global Arguments Tflat {_} _.
 Global Arguments Const {_ _ _ _ _} _.
 Global Arguments Var {_ _ _ _ _} _.
 Global Arguments Op {_ _ _ _ _ _} _ _.
 Global Arguments LetIn {_ _ _ _ _} _ {_} _.
 Global Arguments MatchPair {_ _ _ _ _ _} _ {_} _.
+Global Arguments Fst {_ _ _ _ _ _} _.
+Global Arguments Snd {_ _ _ _ _ _} _.
 Global Arguments Pair {_ _ _ _ _} _ {_} _.
-Global Arguments Return {_ _ _ _ _} _.
 Global Arguments Abs {_ _ _ _ _ _} _.
+Global Arguments Return {_ _ _ _ _} _.
 Global Arguments Compile {_ _ _} make_const {t} _ _.
