src/Specific/GF25519Reflective/Reified/Mul.v
@@ -1,17 +1,17 @@
-Require Import Crypto.Specific.GF25519Reflective.CommonBinOp.
+Require Import Crypto.Specific.GF25519Reflective.Common.
 
 Definition rmulZ_sig : rexpr_binop_sig mul. Proof. reify_sig. Defined.
-Definition rmulW := Eval vm_compute in rword_of_Z rmulZ_sig.
-Lemma rmulW_correct_and_bounded_gen : correct_and_bounded_genT rmulW rmulZ_sig.
+Definition rmulZ := Eval vm_compute in proj1_sig rmulZ_sig.
+Lemma rmulZ_correct_and_bounded_gen : correct_and_bounded_genT rmulZ rmulZ_sig.
 Proof. rexpr_correct. Qed.
-Definition rmul_output_bounds := Eval vm_compute in compute_bounds rmulW ExprBinOp_bounds.
+Definition rmul_output_bounds := Eval vm_compute in compute_bounds rmulZ ExprBinOp_bounds.
 Local Obligation Tactic := intros; vm_compute; constructor.
-Program Definition rmulW_correct_and_bounded
+Program Definition rmulZ_correct_and_bounded
   := ExprBinOp_correct_and_bounded
-       rmulW mul rmulZ_sig rmulW_correct_and_bounded_gen
+       rmulZ mul rmulZ_sig rmulZ_correct_and_bounded_gen
        _ _.
 
 Local Open Scope string_scope.
-Compute ("Mul", compute_bounds_for_display rmulW ExprBinOp_bounds).
-Compute ("Mul overflows? ", sanity_compute rmulW ExprBinOp_bounds).
-Compute ("Mul overflows (error if it does)? ", sanity_check rmulW ExprBinOp_bounds).
+Compute ("Mul", compute_bounds_for_display rmulZ ExprBinOp_bounds).
+Compute ("Mul overflows? ", sanity_compute rmulZ ExprBinOp_bounds).
+Compute ("Mul overflows (error if it does)? ", sanity_check rmulZ ExprBinOp_bounds).
