src/Specific/GF25519Reflective/Reified/Sub.v
@@ -1,12 +1,12 @@
-Require Import Crypto.Specific.GF25519Reflective.CommonBinOp.
+Require Import Crypto.Specific.GF25519Reflective.Common.
 
 Definition rsubZ_sig : rexpr_binop_sig sub. Proof. reify_sig. Defined.
-Definition rsubW := Eval vm_compute in rword_of_Z rsubZ_sig.
-Lemma rsubW_correct_and_bounded_gen : correct_and_bounded_genT rsubW rsubZ_sig.
+Definition rsubZ := Eval vm_compute in proj1_sig rsubZ_sig.
+Lemma rsubZ_correct_and_bounded_gen : correct_and_bounded_genT rsubZ rsubZ_sig.
 Proof. rexpr_correct. Qed.
-Definition rsub_output_bounds := Eval vm_compute in compute_bounds rsubW ExprBinOp_bounds.
+Definition rsub_output_bounds := Eval vm_compute in compute_bounds rsubZ ExprBinOp_bounds.
 
 Local Open Scope string_scope.
-Compute ("Sub", compute_bounds_for_display rsubW ExprBinOp_bounds).
-Compute ("Sub overflows? ", sanity_compute rsubW ExprBinOp_bounds).
-Compute ("Sub overflows (error if it does)? ", sanity_check rsubW ExprBinOp_bounds).
+Compute ("Sub", compute_bounds_for_display rsubZ ExprBinOp_bounds).
+Compute ("Sub overflows? ", sanity_compute rsubZ ExprBinOp_bounds).
+Compute ("Sub overflows (error if it does)? ", sanity_check rsubZ ExprBinOp_bounds).
