src/Specific/GF25519Reflective/Reified/Unpack.v
@@ -1,17 +1,17 @@
-Require Import Crypto.Specific.GF25519Reflective.CommonUnOpWireToFE.
+Require Import Crypto.Specific.GF25519Reflective.Common.
 
 Definition runpackZ_sig : rexpr_unop_WireToFE_sig unpack. Proof. reify_sig. Defined.
-Definition runpackW := Eval vm_compute in rword_of_Z runpackZ_sig.
-Lemma runpackW_correct_and_bounded_gen : correct_and_bounded_genT runpackW runpackZ_sig.
+Definition runpackZ := Eval vm_compute in proj1_sig runpackZ_sig.
+Lemma runpackZ_correct_and_bounded_gen : correct_and_bounded_genT runpackZ runpackZ_sig.
 Proof. rexpr_correct. Qed.
-Definition runpack_output_bounds := Eval vm_compute in compute_bounds runpackW ExprUnOpWireToFE_bounds.
+Definition runpack_output_bounds := Eval vm_compute in compute_bounds runpackZ ExprUnOpWireToFE_bounds.
 Local Obligation Tactic := intros; vm_compute; constructor.
-Program Definition runpackW_correct_and_bounded
+Program Definition runpackZ_correct_and_bounded
   := ExprUnOpWireToFE_correct_and_bounded
-       runpackW unpack runpackZ_sig runpackW_correct_and_bounded_gen
+       runpackZ unpack runpackZ_sig runpackZ_correct_and_bounded_gen
        _ _.
 
 Local Open Scope string_scope.
-Compute ("Unpack", compute_bounds_for_display runpackW ExprUnOpWireToFE_bounds).
-Compute ("Unpack overflows? ", sanity_compute runpackW ExprUnOpWireToFE_bounds).
-Compute ("Unpack overflows (error if it does)? ", sanity_check runpackW ExprUnOpWireToFE_bounds).
+Compute ("Unpack", compute_bounds_for_display runpackZ ExprUnOpWireToFE_bounds).
+Compute ("Unpack overflows? ", sanity_compute runpackZ ExprUnOpWireToFE_bounds).
+Compute ("Unpack overflows (error if it does)? ", sanity_check runpackZ ExprUnOpWireToFE_bounds).
