src/Reflection/Relations.v
@@ -6,31 +6,8 @@ Local Open Scope ctype_scope.
 Section language.
   Context {base_type_code : Type}.
 
-  Let Tbase := (@Tbase base_type_code).
-  Local Coercion Tbase : base_type_code >-> flat_type.
   Local Notation flat_type := (flat_type base_type_code).
   Local Notation type := (type base_type_code).
-
-  Section type.
-    Context (interp_flat_type : flat_type -> Type)
-            (R : forall t, interp_flat_type t -> interp_flat_type t -> Prop).
-    Local Notation interp_type_gen := (interp_type_gen interp_flat_type).
-    Fixpoint interp_type_gen_rel_pointwise (t : type)
-      : interp_type_gen t -> interp_type_gen t -> Prop :=
-      match t with
-      | Tflat t => R t
-      | Arrow _ y => fun f g => forall x, interp_type_gen_rel_pointwise y (f x) (g x)
-      end.
-    Global Instance interp_type_gen_rel_pointwise_Reflexive {H : forall t, Reflexive (R t)}
-      : forall t, Reflexive (interp_type_gen_rel_pointwise t).
-    Proof. induction t; repeat intro; reflexivity. Qed.
-    Global Instance interp_type_gen_rel_pointwise_Symmetric {H : forall t, Symmetric (R t)}
-      : forall t, Symmetric (interp_type_gen_rel_pointwise t).
-    Proof. induction t; simpl; repeat intro; symmetry; eauto. Qed.
-    Global Instance interp_type_gen_rel_pointwise_Transitive {H : forall t, Transitive (R t)}
-      : forall t, Transitive (interp_type_gen_rel_pointwise t).
-    Proof. induction t; simpl; repeat intro; etransitivity; eauto. Qed.
-  End type.
 
   Section flat_type.
     Context {interp_base_type : base_type_code -> Type}
@@ -39,30 +16,27 @@ Section language.
     Fixpoint interp_flat_type_rel_pointwise (t : flat_type)
       : interp_flat_type t -> interp_flat_type t -> Prop :=
       match t with
-      | Syntax.Tbase t => R t
+      | Tbase t => R t
       | Unit => fun _ _ => True
       | Prod _ _ => fun x y => interp_flat_type_rel_pointwise _ (fst x) (fst y)
                                /\ interp_flat_type_rel_pointwise _ (snd x) (snd y)
       end.
-    Definition interp_type_rel_pointwise
-      := interp_type_gen_rel_pointwise _ interp_flat_type_rel_pointwise.
   End flat_type.
 
   Section rel_pointwise2.
     Section type.
       Section hetero.
-        Context (interp_src1 interp_src2 : base_type_code -> Type)
+        Context (interp_src1 interp_src2 : flat_type -> Type)
                 (interp_dst1 interp_dst2 : flat_type -> Type)
                 (Rsrc : forall t, interp_src1 t -> interp_src2 t -> Prop)
                 (Rdst : forall t, interp_dst1 t -> interp_dst2 t -> Prop).
 
-        Fixpoint interp_type_gen_rel_pointwise2_hetero (t : type)
+        Definition interp_type_gen_rel_pointwise2_hetero (t : type)
           : interp_type_gen_hetero interp_src1 interp_dst1 t
             -> interp_type_gen_hetero interp_src2 interp_dst2 t
             -> Prop
           := match t with
-             | Tflat t => Rdst t
-             | Arrow src dst => @respectful_hetero _ _ _ _ (Rsrc src) (fun _ _ => interp_type_gen_rel_pointwise2_hetero dst)
+             | Arrow src dst => @respectful_hetero _ _ _ _ (Rsrc src) (fun _ _ => Rdst dst)
              end.
       End hetero.
       Section homogenous.
@@ -90,7 +64,7 @@ Section language.
         Fixpoint interp_flat_type_rel_pointwise2_gen_Prop (t : flat_type)
           : interp_flat_type interp_base_type1 t -> interp_flat_type interp_base_type2 t -> P
           := match t with
-             | Syntax.Tbase t => R t
+             | Tbase t => R t
              | Unit => fun _ _ => True
              | Prod x y => fun a b => and (interp_flat_type_rel_pointwise2_gen_Prop x (fst a) (fst b))
                                           (interp_flat_type_rel_pointwise2_gen_Prop y (snd a) (snd b))
@@ -109,6 +83,8 @@ Section language.
   End rel_pointwise2.
 
   Section lifting.
+    Let Tbase := (@Tbase base_type_code).
+    Local Coercion Tbase : base_type_code >-> flat_type.
     Section flat_type.
       Context {interp_base_type : base_type_code -> Type}.
       Local Notation interp_flat_type := (interp_flat_type interp_base_type).
@@ -133,6 +109,57 @@ Section language.
         Qed.
       End RProd_iff.
     End flat_type.
+    Section flat_type2.
+      Context {interp_base_type1 interp_base_type2 : base_type_code -> Type}.
+      Lemma lift_interp_flat_type_rel_pointwise2_f_eq {T} (f g : forall t, _ -> T t) t x y
+        : interp_flat_type_rel_pointwise2
+            interp_base_type1 interp_base_type2
+            (fun t x y => f t x = g t y)
+            t x y
+          <-> SmartVarfMap f x = SmartVarfMap g y.
+      Proof.
+        induction t; unfold SmartVarfMap in *; simpl in *; destruct_head_hnf unit; try tauto.
+        rewrite_hyp !*; intuition congruence.
+      Qed.
+      Lemma lift_interp_flat_type_rel_pointwise2_f_eq_id1 (f : forall t, _ -> _) t x y
+        : interp_flat_type_rel_pointwise2
+            interp_base_type1 interp_base_type2
+            (fun t x y => x = f t y)
+            t x y
+          <-> x = SmartVarfMap f y.
+      Proof. rewrite lift_interp_flat_type_rel_pointwise2_f_eq, SmartVarfMap_id; reflexivity. Qed.
+      Lemma lift_interp_flat_type_rel_pointwise2_f_eq_id2 (f : forall t, _ -> _) t x y
+        : interp_flat_type_rel_pointwise2
+            interp_base_type1 interp_base_type2
+            (fun t x y => f t x = y)
+            t x y
+          <-> SmartVarfMap f x = y.
+      Proof. rewrite lift_interp_flat_type_rel_pointwise2_f_eq, SmartVarfMap_id; reflexivity. Qed.
+      Lemma lift_interp_type_rel_pointwise2_f_eq {T} (f g : forall t, _ -> T t) t x y
+        : interp_type_rel_pointwise2
+            interp_base_type1 interp_base_type2
+            (fun t x y => f t x = g t y)
+            t x y
+          <-> (forall a b, SmartVarfMap f a = SmartVarfMap g b -> SmartVarfMap f (x a) = SmartVarfMap g (y b)).
+      Proof.
+        destruct t; simpl; unfold respectful_hetero.
+        setoid_rewrite lift_interp_flat_type_rel_pointwise2_f_eq; reflexivity.
+      Qed.
+      Lemma lift_interp_type_rel_pointwise2_f_eq_id1 (f : forall t, _ -> _) t x y
+        : interp_type_rel_pointwise2
+            interp_base_type1 interp_base_type2
+            (fun t x y => x = f t y)
+            t x y
+          <-> (forall a, x (SmartVarfMap f a) = SmartVarfMap f (y a)).
+      Proof. rewrite lift_interp_type_rel_pointwise2_f_eq; setoid_rewrite SmartVarfMap_id; firstorder (subst; eauto). Qed.
+      Lemma lift_interp_type_rel_pointwise2_f_eq_id2 (f : forall t, _ -> _) t x y
+        : interp_type_rel_pointwise2
+            interp_base_type1 interp_base_type2
+            (fun t x y => f t x = y)
+            t x y
+          <-> (forall a, SmartVarfMap f (x a) = y (SmartVarfMap f a)).
+      Proof. rewrite lift_interp_type_rel_pointwise2_f_eq; setoid_rewrite SmartVarfMap_id; firstorder (subst; eauto). Qed.
+    End flat_type2.
   End lifting.
 End language.
 
@@ -141,7 +168,4 @@ Global Arguments interp_type_gen_rel_pointwise2_hetero {_ _ _ _ _} Rsrc Rdst {t}
 Global Arguments interp_type_gen_rel_pointwise2 {_ _ _} R {t} _ _.
 Global Arguments interp_flat_type_rel_pointwise2_gen_Prop {_ _ _ P} and True R {t} _ _.
 Global Arguments interp_flat_type_rel_pointwise2 {_ _ _} R {t} _ _.
-Global Arguments interp_flat_type_rel_pointwise {_} _ _ {_} _ _.
-Global Arguments interp_type_rel_pointwise {_} _ _ {_} _ _.
-Global Arguments interp_type_gen_rel_pointwise {_ _} _ {_} _ _.
 Global Arguments interp_flat_type_rel_pointwise {_} _ _ {_} _ _.
