src/Specific/GF25519Reflective/Reified/LadderStep.v
@@ -6,11 +6,10 @@ Require Import Crypto.Reflection.Reify.
 Require Import Crypto.Reflection.Syntax.
 Require Import Crypto.Reflection.Relations.
 Require Import Crypto.Reflection.ExprInversion.
-Require Import Crypto.Reflection.Application.
 Require Import Crypto.Reflection.Linearize.
 Require Import Crypto.Reflection.Z.Interpretations64.
 Require Crypto.Reflection.Z.Interpretations64.Relations.
-Require Import Crypto.Reflection.Z.Interpretations64.RelationsCombinations.
+(*Require Import Crypto.Reflection.Z.Interpretations64.RelationsCombinations.*)
 Require Import Crypto.Reflection.Z.Reify.
 Require Export Crypto.Reflection.Z.Syntax.
 Require Import Crypto.Reflection.InterpWfRel.
